Reset after some failed attempts

src/semantics.v
@@ -1,6 +1,7 @@
 Require Import imp.
 Require Import Coq.Init.Nat.
 Require Import Classes.EquivDec.
+Require Import Coq.Arith.Wf_nat.
 
 Notation State := (Var -> nat).
 
@@ -24,24 +25,6 @@ Fixpoint eval_Bexp (b : Bexp) (s : State) : bool :=
   | Or b1 b2 => (eval_Bexp b1 s) || (eval_Bexp b2 s)
   end.
 
-(* Big-step semantics *)
-
-(* We define semantics as a relation as we cannot encode unbounded loops *)
-(* Inductive big_step  *)
-Inductive big_step `{EqDec Var} : Prog -> State -> State -> Prop :=
-| Bskip (s : State) : big_step skip s s
-| Bass (s : State) (v : Var) (a : Aexp) :
-    big_step (ass v a) s (fun x => if x == v then (eval_Aexp a s) else s x)
-| Bseq (s1 s2 s3 : State) (c1 c2 : Prog) (h : big_step c1 s1 s2) : big_step (seq c1 c2) s1 s3
-| BiteT (s1 s2 : State) (b : Bexp) (c1 c2 : Prog) (hb : eval_Bexp b s1 = true)
-    (h : big_step c1 s1 s2) : big_step (ite b c1 c2) s1 s2
-| BiteF (s1 s2 : State) (b : Bexp) (c1 c2 : Prog) (hb : eval_Bexp b s1 = false)
-    (h : big_step c2 s1 s2) : big_step (ite b c1 c2) s1 s2
-| BwhileT (s1 s2 s3 : State) (b : Bexp) (c : Prog) (hb : eval_Bexp b s1 = true)
-    (h1 : big_step c s1 s2) (h2 : big_step (while b c) s2 s3) : big_step (while b c) s1 s3
-| BwhileF (s : State) (b : Bexp) (c : Prog) (hb : eval_Bexp b s = false) : big_step (while b c) s s.
-
-
 (* Small-step semantics *)
 Inductive small_step `{EqDec Var} : (Prog * State) -> (Prog * State) -> Prop :=
 | Sskip (s : State) : small_step (skip, s) (skip, s)
@@ -64,5 +47,44 @@ Inductive small_steps `{EqDec Var} : Prog -> State -> State -> Prop :=
 | Term (s : State) : small_steps skip s s
 | Step (s1 s2 s3 : State) (c1 c2 : Prog) (h1 : small_step (c1, s1) (c2, s2))
     (h2 : small_steps c2 s2 s3) : small_steps c1 s1 s3.
+
+Inductive counting_steps `{EqDec Var} : nat -> Prog -> State -> State -> Prop :=
+| Done (s : State) : counting_steps 0 skip s s
+| Multiple (s1 s2 s3 : State) (c1 c2 : Prog) (n : nat) (h1 : small_step (c1, s1) (c2, s2))
+    (h2 : counting_steps n c2 s2 s3) : counting_steps (1 + n) c1 s1 s3.
+
+Inductive trans `{EqDec Var} : nat -> (Prog * State) -> (Prog * State) -> Prop :=
+| One (s1 s2 : State) (c1 c2 : Prog) (h : small_step (c1, s1) (c2, s2)) : trans 1 (c1, s1) (c2, s2)
+| Trans (s1 s2 s3 : State) (c1 c2 c3 : Prog) (n : nat) (h1 : small_step (c1, s1) (c2, s2))
+    (h2 : trans n (c2, s2) (c3, s3)) : trans (1 + n) (c1, s1) (c3, s3).
+
+(* Big-step semantics *)
+
+(* We define semantics as a relation as we cannot encode unbounded loops *)
+(* Inductive big_step  *)
+Inductive big_step `{EqDec Var} : Prog -> State -> State -> Prop :=
+| Bskip (s : State) : big_step skip s s
+| Bass (s : State) (v : Var) (a : Aexp) :
+    big_step (ass v a) s (fun x => if x == v then (eval_Aexp a s) else s x)
+| Bseq (s1 s2 s3 : State) (c1 c2 : Prog) (h1 : big_step c1 s1 s2) (h2 : big_step c2 s2 s3) :
+    big_step (seq c1 c2) s1 s3
+| BiteT (s1 s2 : State) (b : Bexp) (c1 c2 : Prog) (hb : eval_Bexp b s1 = true)
+    (h : big_step c1 s1 s2) : big_step (ite b c1 c2) s1 s2
+| BiteF (s1 s2 : State) (b : Bexp) (c1 c2 : Prog) (hb : eval_Bexp b s1 = false)
+    (h : big_step c2 s1 s2) : big_step (ite b c1 c2) s1 s2
+| BwhileT (s1 s2 s3 : State) (b : Bexp) (c : Prog) (hb : eval_Bexp b s1 = true)
+    (h1 : big_step c s1 s2) (h2 : big_step (while b c) s2 s3) : big_step (while b c) s1 s3
+| BwhileF (s : State) (b : Bexp) (c : Prog) (hb : eval_Bexp b s = false) : big_step (while b c) s s.
+
+Axiom strong_induction:
+forall P : nat -> Prop,
+(forall n : nat, (forall k : nat, (k < n -> P k)) -> P n) ->
+forall n : nat, P n.
+
+Lemma imp_small_to_big `{EqDec Var} : forall c s1 s2, small_steps c s1 s2 -> big_step c s1 s2.
+Proof. Admitted.
+
+Lemma imp_big_to_small `{EqDec Var} : forall c s1 s2, big_step c s1 s2 -> small_steps c s1 s2.
+Proof. Admitted.
 
 Theorem imp_small_iff_big `{EqDec Var} : forall c s1 s2, big_step c s1 s2 <-> small_steps c s1 s2.
